theories/Dijkstra/StateSpecT.v
@@ -23,6 +23,7 @@ From ITree Require Import
      Core.Divergence
      Dijkstra.DijkstraMonad
      Dijkstra.PureITreeBasics
+     Dijkstra.DelaySpecMonad
    (*  Simple *)
 .
 
@@ -65,11 +66,138 @@ Notation "a ∋ b" := (proj1_sig a b) (at level 70).
 Section StateSpecT.
   Context (S : Type).
   Context (W : Type -> Type).
+  Context {MonadW : Monad W}.
+  Context {OrderW : OrderM W}.
+  Context {OrderedMonadW : OrderedMonad W}.
 
-  Context {SpecMonadW : SpecMonad W}.
+  Definition StateSpecT (A : Type) := stateT S W A.
+  
+  Global Instance StateSpecTOrder : OrderM StateSpecT := 
+    fun A (w1 w2 : stateT S W A) => forall (s : S), w1 s <≈ w2 s.
 
-  Definition StateSpecT (A : Type) := S -> Input W (S *A) -> Prop.
+  Global Instance StateSpecTOrderedLaws : OrderedMonad StateSpecT.
+  Proof.
+    intros A B w1 w2 f1 f2 Hlw Hlf. unfold StateSpecT in *.
+    red in OrderedMonadW. rename OrderedMonadW into HW. repeat red.
+    intros. apply HW; auto. intros. destruct a as [s' a]. simpl.
+    repeat red in Hlf. apply Hlf.
+  Qed.
+  
+  (*Can I encode a pre post thing, state spec enriches the precondition and 
+     specializes post condition*)
+
+  (*maybe I need a computational monad M with a monad iter structure,
+    I think the taus only showed up because I was using hte monad iter structure
+    of strong bisimulation not weak,
+    also note that this loop invar stuff, while relevant to D monads, is not
+    itself of D monads 
+   *)
 
 End StateSpecT.
 
+Section LoopInvarSpecific.
+  Context (S : Type).
+
+  Definition StateSpec (A : Type) := StateSpecT S DelaySpec A.
+
+  Definition State (A : Type) := stateT S Delay A.
+
+  Instance StateIter : MonadIter State := MonadIter_stateT0.
+  
+  Definition reassoc {A B : Type} (t : Delay (S * (A + B) ) ) : Delay ((S * A) + (S * B)  ) :=
+    t >>= (fun '(s,ab) => 
+             match ab with
+             | inl a => ret (inl (s , a))
+             | inr b => ret (inr (s , b))
+             end
+).
+
+  Definition iso_arrow {A B : Type} (f : A -> State B) (g : (S * A) -> Delay (S * B) ) :=
+    forall (a : A) (s : S), f a s ≈ g (s,a).
+
+  Definition decurry_flip {A B C : Type} (f : A -> B -> C) : B * A -> C :=
+    fun '(b,a) => f a b.
+
+  (*this is just decurry*)
+  Definition iso_destatify_arrow {A B : Type} (f : A -> State (A + B) ) : (S * A) -> Delay ((S * A) + (S * B)) :=
+    fun '(s,a) => reassoc (f a s).
+
+
+  
+  (*should be able to use original*)
+  Lemma loop_invar_state: forall (A B : Type) (g : A -> State (A + B)) (a : A) (s : S)
+               (p : Delay ( S * B) -> Prop) (q : Delay ((S * A) + (S *B))  -> Prop  ) 
+               (Hp : resp_eutt _ _ p) (Hq : resp_eutt _ _ q) ,
+        (q (reassoc (g a s) )) -> 
+        (q -+> p) -> (forall t, q t -> q (t >>= (iter_lift ( iso_destatify_arrow g)  ))) -> 
+         (p \1/ divergence) (iter g a s) .
+  Proof.
+    intros. specialize (loop_invar (S * A) (S * B) ) as Hloop.
+    set (iso_destatify_arrow g) as g'.
+    enough ((p \1/ divergence) (KTree.iter g' (s,a) )).
+    - assert (KTree.iter g' (s,a) ≅ iter g a s).
+      + unfold g', iso_destatify_arrow.
+        unfold iter, Iter_Kleisli, Basics.iter, MonadIterDelay, StateIter,
+        MonadIter_stateT0, reassoc.
+        admit. (*obviously the same but something annoying going on*)
+      + assert (Hpdiv : resp_eutt _ _ (p \1/ divergence)).
+        { intros t1 t2 Heutt. split; intros; basic_solve.
+          - left. eapply Hp; eauto. symmetry. auto.
+          - right. rewrite <- Heutt. auto.
+          - left. eapply Hp; eauto.
+          - right. rewrite Heutt. auto.
+         }
+        eapply Hpdiv; try apply H2. rewrite H3. reflexivity.
+     - eapply Hloop; eauto.
+  Admitted.
+
+End LoopInvarSpecific.
+
+Section LoopInvarGeneral.
+  Context (S : Type).
+  Context (M : Type -> Type).
+  Context {MonadM : Monad M}.
+  Context {EqMM : EqM M}.
+  Context {MonadLawsM : MonadLaws M}.
+  Context {IterM : MonadIter M}.
+
+  Context (divergence : forall {A : Type}, M A -> Prop).
+
+  Definition loop_invar_imp {A B : Type} (q : M (A + B) -> Prop ) (p : M B -> Prop) :Prop :=
+    forall m, q (m >>= fun b => ret (inr b) ) -> p m. 
+
+  Definition iter_lift {A B : Type} (g : A -> M (A + B)) : (A + B) -> M (A + B) :=
+    fun x => match x with 
+             | inl a => g a
+             | inr b => ret (inr b) end.
+
+  Notation "q -+> p" := (loop_invar_imp q p) (at level 80).
+
+  Definition resp_eq {A : Type} (p : M A -> Prop) : Prop :=
+    forall m1 m2, m1 ≈ m2 -> (p m1) <-> (p m2).
+(*
+  Definition loop_invar_prop : Prop :=   forall (A B : Type) (g : A -> M (A + B) ) (a : A) 
+                          (p : M B -> Prop) (Hp : resp_eq p)
+                          (q : M (A + B) -> Prop ) (Hq : resp_eq q ),
+    (q -+> p) -> (q (g a)) -> 
+    (forall t, q t ->  q (bind t (iter_lift g))) ->
+    p \1/ divergence) (iter g a).
+
+  Context (divergence : forall (A : Type), M A -> Prop ).
+  (* Context (under_loop_invar : forall (A B : Type) (g : A -> M (A + B) ) (a : A), ) *)
+  (*might need a proof that if that whole inl wf thing happens then it 
+    is some infinite element, or have some kind of underlying loop invariant principle*)
+  (*divergent elements follow two laws bind spin f eq spin, 
+    if
+   *)
+  (*complication, delay monad is simple in some sense, every element is either spin,
+    or it is ret some value*)
+  (*notions of divergence always makes sense in the base monad*)
+
+
+  *)
+
+  
+
+End LoopInvarGeneral.
 
