theories/Dijkstra/ExcSpecT.v
@@ -1,0 +1,70 @@
+From Coq Require Import
+     Arith.PeanoNat
+     Lists.List
+     Strings.String
+     Morphisms
+     Setoid
+     RelationClasses
+     Logic.Classical_Prop
+.
+
+From ExtLib Require Import
+     Data.String
+     Structures.Monad
+     Structures.Traversable
+     Data.List.
+
+From ITree Require Import
+     ITree
+     ITreeFacts
+     Events.MapDefault
+     Events.State
+     Events.StateFacts
+     Core.Divergence
+     Dijkstra.DijkstraMonad
+     Dijkstra.PureITreeBasics
+   (*  Simple *)
+.
+
+From Paco Require Import paco.
+
+Import Monads.
+Import MonadNotation.
+Local Open Scope monad_scope.
+
+Section ExcT.
+  Context (E : Type).
+  Context (W : Type -> Type).
+  Context {MonadW : Monad W}.
+  Context {OrderW : OrderM W}.
+  Context {OrderedMonadW : OrderedMonad W}.
+  
+  Definition ExcSpecT (A : Type) := W (E + A).
+
+  Definition ret_exc (A : Type) (a : A) :ExcSpecT A := ret (inr a).
+
+  Definition bind_exc (A B : Type) (m : W (E + A)) (f : A -> ExcSpecT B) : ExcSpecT B :=
+    bind m  (fun (x : E + A) => match x with inr a => f a | inl e => ret (inl e) end). 
+
+  Global Instance ExcSpecTMonad : Monad ExcSpecT :=
+    {
+      ret := ret_exc;
+      bind := bind_exc
+    }.
+
+  Global Instance ExcSpecTOrder : OrderM ExcSpecT :=
+    fun _ w1 w2 => OrderW _ w1 w2.
+
+  
+
+   Global Instance ExcSpecTOrderedLaws : OrderedMonad ExcSpecT.
+   Proof.
+     rename OrderedMonadW into Hw. intros A B w1 w2 f1 f2 Hlw Hlf.
+     red in Hw. apply Hw; auto. intros. destruct a as [e |  a]. simpl.
+     - admit. (*forgot to add some basic partial order laws*)
+     - apply Hlf.
+   Admitted.
+
+
+
+End ExcT.
